## Recursively Defined Functions

**Definition:** A _recursive_ or _inductive_ definition of a function consists of two steps:

. **Basis Step:** Specify the value of the function at zero
2. **Recursive Step:** Give a rule for finding its value at an integer from its values at smaller integers

A function $f(n)$ is the same as a sequence $a_{0},a_{1},\dots,$ where $a_{i}$, where $f(i)=a_{i}$. This was done using recurrence relations in [[(M.3.4.1a) Sequences]].

#### Examples

**Problem 1:** Suppose $f$ is defined by:\
$f(0)=3$,\
$f(n+1)=2f(n)+3$

Find $f(1),f(2),f(3),f(4)$

**Solution:**
- $f(1)=2f(0)+3=2 \times 3+3=9$
- $f(2)=2f(1)+3=2 \times 9+3=21$
- $f(3)=2f(2)+3=2 \times 21+3=45$
- $f(4)=2f(3)+3=2 \times +3=93$

**Problem 2:** Give a recursive definition of the factorial function $n!$:

**Solution:**

$f(0)=1$\
$f(n+1)=(n+1)\times f(n)$

## Fibonacci Numbers

#### Examples

**Problem 1:** The Fibonacci numbers are defined as follows:\
$f_{0}=0$\
$f_{1}=1$\
$f_{n}=f_{n-1}+f_{n-2}$

Find $f_{2},f_{3},f_{4},f_{5}$

**Solution:**
- $f_{2}=f_{1}+f_{0}=1+0=1$
- $f_{3}=f_{2}+f_{1}=1+1=2$
- $f_{4}=f_{3}+f_{2}=2+1=3$
- $f_{5}=f_{4}+f_{3}=3+2=5$

**Problem 2:** Show that whenever $n\geq3,~f_{n}>\alpha^{n-2}$, where $\alpha=\frac{(1+ \sqrt{5})}{2}$

**Solution:** Let $P(n)$ be the statement $f_{n}>\alpha^{n-2}$. Use strong induction to show that $P(n)$ is true whenever $n\geq3$

- **Basis Step:** $P(3)$ holds since $\alpha<2=f_{3}$ and $P(4)$ holds since $\alpha^{2}=\frac{(3+\sqrt{5})}{2}<3=f_{4}$
- **Inductive Step:** Assume that $P(j)$ holds, i.e., $f_{j}>\alpha^{j-2}$ for all integers $j$ with $3 \leq j \leq k$, where $k\geq4$. Show that $P(k+1)$ holds, i.e., $f_{k+1}>\alpha^{k-1}$.
  - Since $\alpha^{2}=\alpha+1$ (because $\alpha$ is a solution of $x^{2}-x-1=0$), 
$$\alpha^{k-1}=\alpha^{2} \times \alpha^{k-3}=(\alpha+1) \times \alpha^{k-3}+1 \times \alpha^{k-3}=\alpha^{k-2}+\alpha^{k-3}$$
  - By the inductive hypothesis, $k\geq4$, meaning
$$f_{k-1}>\alpha^{k-3},~~~~f_{k}>\alpha^{k-2}$$
  - Therefore, it follows that 
$$f_{k+1}=f_{k}+f_{k-1}>\alpha^{k-2}+\alpha^{k-3}=\alpha^{k-1}$$
  - Hence, $P(k+1)$ is true

## Recursively Defined Sets and Structures

Recursive definitions of sets have two parts:

1. The **basis step** specifies an initial collection of elements
2. The **recursive step** gives the rules for forming new elements in the set from those already known to be in the set.

Sometimes the recursive definition has an **exclusion rule**, which specifies that the set contains nothing other than those elements specified in the basis step and generated by application of the rules in the recursive step.

We will always assume that the exclusion rule holds, even if it is not explicitly mentioned.

Later, we'll develop a form of induction, called **structural induction**, to prove results about recursively defined sets.

#### Examples

**Problem 1:** Subset of integers $S$:
- **Basis Step:** $3 \in S$
- **Recursive Step:** If $x \in S$ and $y \in S$, then $x+y$ is in $S$

Initially, 3 is in $S$, then $3+3=6$, then $3+6=9$, etc.

**Problem 2:** Natural numbers $N$
- **Basis Step:** $0 \in N$
- **Recursive Step:** If $n$ is in $N$, then $n+1$ is in $N$

Initially, 0 is in $N$, then $0+1=1$, then $1+1=2$, etc.

## Strings

**Definition:** The set $\sum^{*}$ of strings over the alphabet $\sum$:
- **Basis Step:** $\lambda \in \sum^{*}$ ($\lambda$ is the empty string)
- **Recursive Step:** If $w$ is in $\sum^{*}$ and $x$ is in $\sum$, then $wx \in \sum^{*}$

##### Examples

Examples include
- If $\sum=\{0,1\}$, the strings in $\sum^{*}$ are the set of all bit strings, $\lambda,0,1,00,01,10,11$, etc.
- If $\sum=\{a,b\}$, show that $aab$ is in $\sum^{*}$
  - Since $\lambda \in \sum^{*}$ and $a \in \sum,~ a \in \sum^{*}$
  - Since $a \in \sum^{*}$ and $a \in \sum,~ aa \in \sum^{*}$
  - Since $aa \in \sum^{*}$ and $b \in \sum,~ aab \in \sum^{*}$

### String Concatenation

**Definition:** Two strings can be combined via the operation of **concatenation**. Let $\sum$ be a set of symbols and $\sum^{*}$ be the set of strings formed from the symbols in $\sum$. We can define the concatenation of two strings, denoted by $\cdot$, recursively as follows.

- **Basis Step:** If $w \in \sum^{*}$, then $w \cdot \lambda=w$
- **Recursive Step:** If $w_{1} in \sum^{*}$ and $w_{2} \in \sum^{*}$ and $x \in \sum$, then $w_{1} \cdot (w_{2}x)=(w_{1} \cdot w_{2})x$

Often, $w_{1} \cdot w_{2}$ is written as $w_{1}w_{2}$. So, if $w_{1}=$ abra and $w_{2}=$ cadabra, the concatenation would be $w_{1}w_{2}=$ abracadabra.

### Length of a String

#### Example

**Problem:** Give a recursive define of $l(w)$, the length of string $w$.

**Solution:** The length of a string can be recursively defined by:\
$l(\lambda)=0$;\
$l(wx)=l(w)+1$ if $w \in \sum^{*}$ and $x \in \sum$

## Well-Formed Formulae in Propositional Logic

**Definition:** The set of **well-formed formulae** in propositional logic involving **T**, **F**, propositional variables and operators from the set $\{\neg, \land, \lor, \to, \leftrightarrow\}$.

- **Basis Step:** **T**, **F**, and $s$, where $s$ is a propositional variable, are well-formed formulae
- **Recursive Step:** If $E$ and $F$ are well-formed form, then $(\neg E),(E \land F),(E \lor F), (E \to F), (E \leftrightarrow F)$, are well-formed formulae.

##### Examples
- $((p \lor q) \to (q \land F))$ is a well-formed formula
- $pq \land$ is **not** a well-formed formula

## Rooted Trees

**Definition:** The set of **rooted trees**, where a rooted tree consists of a set of vertices containing a distinguished vertex called the **root**, and edges connecting these vertices, can be defined recursively by these steps:

- **Basis Step:** A single vertex $r$ is a rooted tree
- **Recursive Step:** Suppose that $T_{1},T_{2},\dots,T_{n}$ are disjoint rooted trees with roots $r_{1},r_{2},\dots,r_{n}$, respectively. Then the graph formed by starting with a root $r$, which is not in any of the rooted trees $T_{1},T_{2},\dots,T_{n}$, and adding an edge from $r$ to each of the vertices $r_{1},r_{2},\dots,r_{n}$ is also a rooted tree.

## Full Binary Trees

**Definition:** The set of **full binary trees** can be defined recursively by these steps:

- **Basis Step:** There is a full binary tree consisting of only a single vertex $r$
- **Recursive Step:** If $T_{1}$ and $T_{2}$ are disjoint full binary trees, there is a full binary tree, denoted by $T_{1} \cdot T_{2}$, consisting of a root $r$ together wit edges connecting the root to each of the roots of the left subtree $T_{1}$ and the right subtree $T_{2}$

## Induction and Recursively Defined Sets

#### Example

**Problem:** Show that the set $S$ defined by specifying that $3 \in S$ and that if $x \in S$, then $x+y$ is in $S$, is the set of all positive integers that are multiples of 3.

**Solution:** Let $A$ be the set of all positive integers divisible by 3. To prove that $A=S$, show that $A$ is a subset of $S$ and $S$ is a subset of $A$.

- $A$ is a subset of $S$: Let $P(n)$ be the statement that $3n$ belongs to $S$:
  - **Basis Step:** $3 \times 1=3 \in S$, by the first part of the recursive definition.
  - **Inductive Step:** Assume $P(k)$ is true. By the second part of the recursive definition, if $3k \in S$, then since $3 \in S,~3k+3=3(k+1) \in S$. Hence, $P(k+1)$ is true.

- $S$ is a subset of $A$:
  - **Basis Step:** $3 \in S$ by the first part of the recursive definition, and $3=3\times1$
  - **Inductive Step:** The second part of the recursive definition adds $x+y$ to $S$, if both $x$ and $y$ and in $S$. If $x$ and $y$ are both in $A$, then both $x$ and $y$ are divisible by 3. Thus, it follows that $x+y$ is divisible by 3.
