## Linear Transformations in General Vector Spaces

Given the vector spaces $V$ and $W$, the transformation $F:V \to W$, which assigns a single vector $F(\vec{u})$ in $W$ to every vector $u$ in $V$, is said to be a _linear transformation_ if
1. For any vectors $\vec{u}$, $\vec{v}$ in $V$, $F(\vec{u}+\vec{v})=F(\vec{u})+F(\vec{v})$  and
2. For any vector $\vec{u}$ in $V$ and scalar $c$, $F(c \vec{u})=cF(\vec{u})$
This vector $F(\vec{u})$ is called the _image_ of $u$ under the transformation $F$.

### Condition 1

![](linear_transformation_part1.png)

### Condition 2

![](linear_transformation_part2.png)

### Theorem 5.1

If $F:V \to W$ is a linear transformation and $V,W$ are vector spaces then

a. $F(\vec{0})=\vec{0}$ and
b. $F(c_{1} \vec{u_{1}}+\dots+c_{k} \vec{u_{k}})=c_{1} F(\vec{u_{1}})+\dots+c_{k} F(\vec{u_{k}})$

### Example 1

Determine if $F:M_{nn} \to M_{nn}$ defined by $F(A)=A^T$ is a linear transformation.

#### Solution

1. For any vectors $\vec{u},\vec{v}$ in $V,F(\vec{u}+\vec{v})=F(\vec{u}+\vec{v})=F(\vec{u})+F(\vec{v})$
	- $LHS=F(A+B)=(A+B)^T$
	- $RHS=F(A)+F(B)=A^T+B^T$
		- These are both equivalent by _Theorem 1.4 part 1_

2. For any vector $\vec{u}$ in $V$ and scalar $c,F(c \vec{u})=cF (\vec{u})$
	- $LHS=F(cA)=(cA)^T$
	- $RHS=cF(A)=cA^T$
		- These are both equivalent by _Theorem 1.4 part 2_

Thus, $F$ is a linear transformation

### Example 2

Determine if $F_{2}(\begin{bmatrix}x \\ y\end{bmatrix})=\begin{bmatrix}x^2 - y^2 \\ xy \\ x\end{bmatrix}$ is a linear transformation.

#### Solution

1. For any vectors $\vec{u},\vec{v}$ in $V,F(\vec{u}+\vec{v})=F(\vec{u}+\vec{v})=F(\vec{u})+F(\vec{v})$
	- $LHS=F_{2}(\vec{u}+\vec{v})=F_{2}(\begin{bmatrix}1 \\ 0\end{bmatrix}+\begin{bmatrix}0 \\ 1\end{bmatrix})=F_{2}(\begin{bmatrix}1 \\ 1\end{bmatrix})= \begin{bmatrix}1^2 - 1^2 \\ 1 \times 1 \\ 1\end{bmatrix} = \begin{bmatrix}0 \\ 1 \\ 1\end{bmatrix}$
	- $RHS=F_{2} (\vec{u})+F_{2}(\vec{v})=F_{2} (\begin{bmatrix}1 \\ 0\end{bmatrix})+F_{2} (\begin{bmatrix}0 \\ 1\end{bmatrix})=\begin{bmatrix}1 \\ 0 \\ 1\end{bmatrix}+\begin{bmatrix}-1 \\ 0 \\ 0\end{bmatrix}=\begin{bmatrix}0 \\ 0 \\ 1\end{bmatrix}$

These two vectors are _not_ equivalent, meaning they are not a linear transformation.

### Example 3

Determine if $F(a_{0}+a_{1} t+a_{2}t^t + a_{3}t^3 + a_{4}t^4)= \begin{bmatrix}a_{0}+2a_{2} & 0 \\ a_{0}-4a_{4} & a_{2}+2a_{4}\end{bmatrix}$ is a linear transformation.

#### Solution

1. For any vectors $\vec{u},\vec{v}$ in $V,F(\vec{u}+\vec{v})=F(\vec{u})+F(\vec{v})$

$$
LHS=F((a_{0}+a_{1}t + a_{2}t^2 + a_{3}t^3 +a_{4} t^4)+(b_{0} + b_{1}t + b_{2}^2 + b_{3}^3 + b_{4}t^4))
$$

$$
=F((a_{0}+b_{0})+(a_{1} + b_{1})t + (a_{2}+b_{2})t^2 + (a_{3}+b_{3})t^3+(a_{4}+b_{4})t^4)
$$

$$
=
\begin{bmatrix}
a_{0} + b_{0} + 2(a_{2} + b_{2}) & 0 \\
a_{0} + b_{0} - 4(a_{4}+b_{4}) & a_{2}+b_{2}+2(a_{4}+b_{4})
\end{bmatrix}
$$

$$
RHS=F(a_{0}+a_{1}t + a_{2}t^2 a_{3}t^3 + a_{4}t^4)+F(b_{0}+b_{1}t + b_{2}t^2 + b_{3}t^3+ b_{4}t^4)
$$

$$
=
\begin{bmatrix}
a_{0} + 2a_{2} & 0 \\
a_{0} - 4a_{4} & a_{2}+2a_{4}
\end{bmatrix}
+
\begin{bmatrix}
b_{0} + 2b_{2} & 0 \\
b_{0} -4b_{4} & b_{2}+2b_{4}
\end{bmatrix}
$$

$$
=
\begin{bmatrix}
a_{0}+b_{0} + 2(a_{2} + b_{2}) & 0 \\
a_{0}+b_{0} - 4(a_{4}+b_{4}) & a_{2}+b_{2}+2(a_{4} + b_{4})
\end{bmatrix}
\quad
=
LHS
$$


2. For any vector $\vec{u}$ in $V$ and scalar $c,F(c \vec{u})=cF(\vec{u})$

$$
LHS = F(c(a_{0}+a_{1}t + a_{2}t^2 + a_{3}t^3 + a_{4}t^4))
$$

$$
= F(ca_{0} + ca_{1} t + ca_{2} t^2 + ca_{3} t^3 + ca_{4} t^4)
$$

$$
=
\begin{bmatrix}
ca_{0} + 2ca_{2} & 0 \\
ca_{0} - 4ca_{4} & ca_{2} + 2ca_{4}
\end{bmatrix}
$$

$$
cF(a_{0} + a_{1} t + a_{2}t^2 + a_{3}t^3 + a_{4}t^4)
\quad
=
RHS
$$

Both conditions hold, so this is a linear transformation. 

### Example 4

Is $F(a_{0}+ a_{1}t + a_{2}t^2a+ a_{3}t^3 + a_{4}t^4)=\begin{bmatrix}a_{0} + 2a_{2} & 0 \\ a_{0}-4a_{4} & a_{2}+2a_{4}\end{bmatrix}$ a linear transformation?

#### Solutions

1. For any vectors $\vec{u},\vec{v}$ in $V,F(\vec{u}+\vec{v})=F(\vec{u})+F(\vec{v})$

$$
RHS=F(a_{0}+a_{1}t + a_{2}t^2 + a_{3}t^3 + a_{4}t^4)+F(b_{0}+b_{1}t + b_{2}t^2 + b_{3}t^3 + b_{4}t^4)
$$

$$
=\begin{bmatrix}a_{0} + 2a_{2} & 0 \\ a_{0}-4a_{4} & a_{2} + 2a_{4}\end{bmatrix}+ \begin{bmatrix}b_{0}+2b_{2} & 0 \\ b_{0}-4b_{4} & b_{2} + 2b_{4}\end{bmatrix}
$$

$$
=
\begin{bmatrix}
a_{0}+b_{0}+2(a_{2}+b_{2}) & 0 \\
a_{0} + b_{0} - 4(a_{4}+b_{4} & a_{2}+b_{2}+2(a_{4} + b_{4}))
\end{bmatrix}
\quad
=
LHS
$$

2. For any vector $\vec{u}$ in $V$ and scalar $c,F(c \vec{u})=cF(\vec{u})$

$$
LHS= F(c(a_{0}+a_{1} t + a_{2}t^2 + a_{3}t^3 + a_{4}t^4))
$$

$$
= F(c a_{0} + c a_{1} t + a_{2}t^2 + a_{3}t^3 + a_{4}t^4))
$$

$$
=
\begin{bmatrix}
ca_{0} + 2ca_{2} & 0 \\
ca_{0} - 4ca_{4} & ca_{2} + 2ca_{4}
\end{bmatrix}
$$

$$
=
c
\begin{bmatrix}
a_{0} + 2a_{2} & 0 \\
a_{0} - 4a_{4} & a_{2} + 2a_{4}
\end{bmatrix}
$$

$$
cF(a_{0} + a_{1}t + a_{2}t^2 + a_{3}t^3 + a_{4}t^4)
$$

Therefore, this is a linear transformation.

### Theorem 5.2

If $V_{1},V_{2},$ and $V_{3}$ are vector spaces and $F:V_{1} \to V_{2}, ~ G:V_{2} \to V_{3}$ are linear transformations then $H:V_{1} \to V_{3}$ defined by $H(\vec{u})=G(F(\vec{u}))$ is also a linear transformation.
