## Summation
- Sum of the terms $a_{m},a_{m+1},\dots,a_{n}$ from the sequence $\{a_{n}\}$
- Either one of the following notations:

$$\sum_{j=m} ^n  a_{j}$$

$$\sum m\leq j\leq n~~~a_{j}$$

More generally for a set $S$

$$\sum j \in S~~a_{j}$$

- - -

### Geometric Series

Sums of terms of geometric expressions:

![[geometric_series.png]]

**Proof for Case 1:** If r=1,
$\sum_{j=0} ^n  ar^{j}=\sum_{j=0}^n a=(n+1)a$                 if r =1

**Proof for Case 2**: If $r \neq 1$

To compute the summation $S_{n}$. First, multiply both sides of the equality by $r$, then manipulate the resulting some as:

$S_{n}=\sum_{j=0}^nar^j$ 

$rS_{n}=r\sum_{j=0}^nar^j$

$= \sum_{j=0}^nar^j+1$

Replacing the index of summation with $k=j+1$:

$= \sum_{k=1}^{n+1}ar^k$       

Separating the last term $k=n+1$ and subtracting the first term $k=0$:
$\left( \sum_{k=0} ^n ar^k \right)+(ar^{n+1}-a)$

Substituting S for for the summation formula
$= S_{n}+(ar^{n+1}-a)$ 

$\therefore rS_{n}=S_{n}+(ar^{n+1}-a)$

or $S_{n}=\frac{ar^{n+1}-a}{r-1}$    if $r \neq 1$








